spec/sail/lean/Out.lean
@@ -15,6 +15,7 @@ namespace Out.Functions
 
 open option
 open VBitOp
+open TLBIOperationTarget
 open MemBarrierOp
 open MBReqTypes
 open MBReqDomain
@@ -22,7 +23,7 @@ open LogicalOp
 open CompareOp
 open BarrierExecutionTarget
 
-/-- Type quantifiers: k_ex9962_ : Bool, k_ex9961_ : Bool -/
+/-- Type quantifiers: k_ex10719_ : Bool, k_ex10718_ : Bool -/
 def neq_bool (x : Bool) (y : Bool) : Bool :=
   (! (x == y))
 
@@ -172,7 +173,7 @@ def ConditionHolds (cond : (BitVec 4)) (nzcv : (BitVec 4)) : Bool :=
   then (! result)
   else result
 
-/-- Type quantifiers: k_ex10146_ : Bool, k_ex10145_ : Bool, k_datasize : Nat, k_datasize ∈
+/-- Type quantifiers: k_ex10903_ : Bool, k_ex10902_ : Bool, k_datasize : Nat, k_datasize ∈
   {32, 64} -/
 def integer_conditional_select (condition : (BitVec 4)) (nzcv : (BitVec 4)) (else_inc : Bool) (else_inv : Bool) (operand1 : (BitVec k_datasize)) (operand2 : (BitVec k_datasize)) : (BitVec k_datasize) :=
   let result : (BitVec k_datasize) := operand2
@@ -188,7 +189,7 @@ def integer_conditional_select (condition : (BitVec 4)) (nzcv : (BitVec 4)) (els
     then (BitVec.addInt result 1)
     else result)
 
-/-- Type quantifiers: k_ex10162_ : Bool, k_datasize : Nat, k_datasize ∈ {32, 64} -/
+/-- Type quantifiers: k_ex10919_ : Bool, k_datasize : Nat, k_datasize ∈ {32, 64} -/
 def integer_conditional_compare_register (condition : (BitVec 4)) (nzcv : (BitVec 4)) (flags__arg : (BitVec 4)) (operand1 : (BitVec k_datasize)) (operand2__arg : (BitVec k_datasize)) (sub_op : Bool) : (BitVec 4) :=
   let flags : (BitVec 4) := flags__arg
   let operand2 : (BitVec k_datasize) := operand2__arg
@@ -333,7 +334,7 @@ def vector_transfer_integer_dup (datasize : Nat) (elements : Nat) (esize : Nat) 
     loop_vars := (aset_Elem result e esize element)
   (pure loop_vars)
 
-/-- Type quantifiers: k_ex10301_ : Bool, datasize : Nat, elements : Nat, esize : Nat, esize ≥ 1
+/-- Type quantifiers: k_ex11058_ : Bool, datasize : Nat, elements : Nat, esize : Nat, esize ≥ 1
   ∧ elements ≥ 1 ∧ (elements * esize) = datasize -/
 def vector_arithmetic_binary_uniform_add_wrapping_single (datasize : Nat) (elements : Nat) (esize : Nat) (operand1 : (BitVec datasize)) (operand2 : (BitVec datasize)) (sub_op : Bool) : (BitVec datasize) := Id.run do
   let result : (BitVec datasize) := (Zeros datasize)
@@ -356,7 +357,7 @@ def vector_arithmetic_binary_uniform_add_wrapping_single (datasize : Nat) (eleme
     (pure loop_vars) ) : Id ((BitVec esize) × (BitVec esize) × (BitVec datasize)) )
   (pure result)
 
-/-- Type quantifiers: k_ex10369_ : Bool, k_ex10368_ : Bool, datasize : Nat, elements : Nat, esize :
+/-- Type quantifiers: k_ex11126_ : Bool, k_ex11125_ : Bool, datasize : Nat, elements : Nat, esize :
   Nat, esize ≥ 1 ∧ elements ≥ 1 ∧ (elements * esize) = datasize -/
 def vector_arithmetic_binary_uniform_maxmin_single (datasize : Nat) (elements : Nat) (esize : Nat) (operand1 : (BitVec datasize)) (operand2 : (BitVec datasize)) (minimum : Bool) (is_unsigned : Bool) : (BitVec datasize) := Id.run do
   let result : (BitVec datasize) := (Zeros datasize)
@@ -381,7 +382,7 @@ def vector_arithmetic_binary_uniform_maxmin_single (datasize : Nat) (elements : 
     (pure loop_vars) ) : Id (Int × Int × Int × (BitVec datasize)) )
   (pure result)
 
-/-- Type quantifiers: k_ex10420_ : Bool, k_ex10419_ : Bool, datasize : Nat, elements : Nat, esize :
+/-- Type quantifiers: k_ex11177_ : Bool, k_ex11176_ : Bool, datasize : Nat, elements : Nat, esize :
   Nat, esize ≥ 1 ∧ elements ≥ 1 ∧ (elements * esize) = datasize -/
 def vector_arithmetic_binary_uniform_cmp_int (cmp_eq : Bool) (datasize : Nat) (elements : Nat) (esize : Nat) (operand1 : (BitVec datasize)) (operand2 : (BitVec datasize)) (is_unsigned : Bool) : (BitVec datasize) := Id.run do
   let result : (BitVec datasize) := (Zeros datasize)
@@ -410,7 +411,7 @@ def vector_arithmetic_binary_uniform_cmp_int (cmp_eq : Bool) (datasize : Nat) (e
     (pure loop_vars) ) : Id (Int × Int × (BitVec datasize) × Bool) )
   (pure result)
 
-/-- Type quantifiers: k_ex10466_ : Bool, datasize : Nat, elements : Nat, esize : Nat, esize ≥ 1
+/-- Type quantifiers: k_ex11223_ : Bool, datasize : Nat, elements : Nat, esize : Nat, esize ≥ 1
   ∧ elements ≥ 1 ∧ (elements * esize) = datasize -/
 def vector_arithmetic_binary_uniform_cmp_bitwise (and_test : Bool) (datasize : Nat) (elements : Nat) (esize : Nat) (operand1 : (BitVec datasize)) (operand2 : (BitVec datasize)) : (BitVec datasize) := Id.run do
   let result : (BitVec datasize) := (Zeros datasize)
@@ -489,7 +490,7 @@ def vector_arithmetic_unary_cmp_int_bulk (comparison : CompareOp) (datasize : Na
     (pure loop_vars) ) : Id (Int × (BitVec datasize) × Bool) )
   (pure result)
 
-/-- Type quantifiers: k_ex10595_ : Bool, datasize : Nat, elements : Nat, esize : Nat, esize ≥ 1
+/-- Type quantifiers: k_ex11352_ : Bool, datasize : Nat, elements : Nat, esize : Nat, esize ≥ 1
   ∧ elements ≥ 1 ∧ (elements * esize) = datasize -/
 def vector_arithmetic_binary_uniform_sub_saturating (datasize : Nat) (elements : Nat) (esize : Nat) (operand1 : (BitVec datasize)) (operand2 : (BitVec datasize)) (is_unsigned : Bool) : (BitVec datasize) := Id.run do
   let result : (BitVec datasize) := (Zeros datasize)
@@ -512,7 +513,7 @@ def vector_arithmetic_binary_uniform_sub_saturating (datasize : Nat) (elements :
     (pure loop_vars) ) : Id (Int × Int × Int × (BitVec datasize)) )
   (pure result)
 
-/-- Type quantifiers: k_ex10646_ : Bool, shift : Int, k_ex10644_ : Bool, k_ex10643_ : Bool, datasize
+/-- Type quantifiers: k_ex11403_ : Bool, shift : Int, k_ex11401_ : Bool, k_ex11400_ : Bool, datasize
   : Nat, elements : Nat, esize : Nat, esize ≥ 1 ∧
   elements ≥ 1 ∧ (elements * esize) = datasize -/
 def vector_shift_right (accumulate : Bool) (datasize : Nat) (elements : Nat) (esize : Nat) (operand : (BitVec datasize)) (accumulator : (BitVec datasize)) (round : Bool) (shift : Int) (is_unsigned : Bool) : (BitVec datasize) := Id.run do
@@ -542,7 +543,7 @@ def vector_shift_right (accumulate : Bool) (datasize : Nat) (elements : Nat) (es
     (pure loop_vars) ) : Id (Int × (BitVec datasize)) )
   (pure result)
 
-/-- Type quantifiers: k_ex10699_ : Bool, datasize : Nat, elements : Nat, elements ≥ 1 ∧
+/-- Type quantifiers: k_ex11456_ : Bool, datasize : Nat, elements : Nat, elements ≥ 1 ∧
   (elements * 8) = datasize ∧ datasize ≤ 128 -/
 def vector_transfer_vector_table (datasize : Nat) (elements : Nat) (is_tbl : Bool) (indices : (BitVec datasize)) (table : (BitVec 128)) (dst : (BitVec datasize)) : (BitVec datasize) := Id.run do
   let result : (BitVec datasize) :=
@@ -566,7 +567,7 @@ def vector_transfer_vector_extract (datasize : Nat) (hi : (BitVec datasize)) (lo
   let concat : (BitVec (2 * datasize)) := (hi +++ lo)
   (BitVec.slice concat position datasize)
 
-/-- Type quantifiers: k_ex10731_ : Bool, k_ex10730_ : Bool, datasize : Nat, elements : Nat, esize :
+/-- Type quantifiers: k_ex11488_ : Bool, k_ex11487_ : Bool, datasize : Nat, elements : Nat, esize :
   Nat, esize ≥ 1 ∧ elements ≥ 1 ∧ (elements * esize) = datasize -/
 def vector_reduce_intmax (datasize : Nat) (elements : Nat) (esize : Nat) (operand : (BitVec datasize)) (min : Bool) (is_unsigned : Bool) : (BitVec esize) := Id.run do
   let maxmin : Int := 0
@@ -622,7 +623,7 @@ def num_of_LogicalOp (arg_ : LogicalOp) : Int :=
   | .LogicalOp_EOR => 1
   | .LogicalOp_ORR => 2
 
-/-- Type quantifiers: k_ex10789_ : Bool, datasize : Nat, datasize ≥ 1 -/
+/-- Type quantifiers: k_ex11546_ : Bool, datasize : Nat, datasize ≥ 1 -/
 def vector_arithmetic_binary_uniform_logical_andorr (datasize : Nat) (invert : Bool) (operand1 : (BitVec datasize)) (operand2__arg : (BitVec datasize)) (op : LogicalOp) : (BitVec datasize) :=
   let operand2 : (BitVec datasize) := operand2__arg
   let result : (BitVec datasize) := (Zeros datasize)
@@ -695,7 +696,7 @@ def FPNeg (op : (BitVec k_N)) : (BitVec k_N) :=
 def FPAbs (op : (BitVec k_N)) : (BitVec k_N) :=
   (0#1 +++ (BitVec.slice op 0 ((Sail.BitVec.length op) -i 1)))
 
-/-- Type quantifiers: k_ex10948_ : Bool, datasize : Nat, elements : Nat, esize : Nat, esize ∈
+/-- Type quantifiers: k_ex11705_ : Bool, datasize : Nat, elements : Nat, esize : Nat, esize ∈
   {32, 64} ∧ elements ≥ 1 ∧ (elements * esize) = datasize -/
 def vector_arithmetic_binary_uniform_add_fp (datasize : Nat) (elements : Nat) (esize : Nat) (operand1 : (BitVec datasize)) (operand2 : (BitVec datasize)) (fpcr : (BitVec 32)) (pair : Bool) : (BitVec datasize) := Id.run do
   let result : (BitVec datasize) := (Zeros datasize)
@@ -725,7 +726,7 @@ def vector_arithmetic_binary_uniform_add_fp (datasize : Nat) (elements : Nat) (e
     (pure loop_vars) ) : Id ((BitVec esize) × (BitVec esize) × (BitVec datasize)) )
   (pure result)
 
-/-- Type quantifiers: k_ex11055_ : Bool, datasize : Nat, elements : Nat, esize : Nat, esize ∈
+/-- Type quantifiers: k_ex11812_ : Bool, datasize : Nat, elements : Nat, esize : Nat, esize ∈
   {32, 64} ∧ elements ≥ 1 ∧ (elements * esize) = datasize -/
 def vector_arithmetic_binary_uniform_sub_fp (datasize : Nat) (elements : Nat) (esize : Nat) (operand1 : (BitVec datasize)) (operand2 : (BitVec datasize)) (fpcr : (BitVec 32)) (abs : Bool) : (BitVec datasize) := Id.run do
   let result : (BitVec datasize) := (Zeros datasize)
@@ -773,7 +774,7 @@ def vector_arithmetic_binary_uniform_mul_fp_product (datasize : Nat) (elements :
     (pure loop_vars) ) : Id ((BitVec esize) × (BitVec esize) × (BitVec datasize)) )
   (pure result)
 
-/-- Type quantifiers: k_ex11229_ : Bool, datasize : Nat, elements : Nat, esize : Nat, esize ∈
+/-- Type quantifiers: k_ex11986_ : Bool, datasize : Nat, elements : Nat, esize : Nat, esize ∈
   {32, 64} ∧ elements ≥ 1 ∧ (elements * esize) = datasize -/
 def vector_arithmetic_binary_uniform_mul_fp_fused (datasize : Nat) (elements : Nat) (esize : Nat) (operand1 : (BitVec datasize)) (operand2 : (BitVec datasize)) (operand3 : (BitVec datasize)) (fpcr : (BitVec 32)) (sub_op : Bool) : (BitVec datasize) := Id.run do
   let result : (BitVec datasize) := (Zeros datasize)
@@ -799,7 +800,7 @@ def vector_arithmetic_binary_uniform_mul_fp_fused (datasize : Nat) (elements : N
     (pure loop_vars) ) : Id ((BitVec esize) × (BitVec esize) × (BitVec datasize)) )
   (pure result)
 
-/-- Type quantifiers: k_ex11305_ : Bool, k_ex11304_ : Bool, datasize : Nat, elements : Nat, esize :
+/-- Type quantifiers: k_ex12062_ : Bool, k_ex12061_ : Bool, datasize : Nat, elements : Nat, esize :
   Nat, esize ∈ {32, 64} ∧ elements ≥ 1 ∧ (elements * esize) = datasize -/
 def vector_arithmetic_binary_uniform_maxmin_fp_1985 (datasize : Nat) (elements : Nat) (esize : Nat) (operand1 : (BitVec datasize)) (operand2 : (BitVec datasize)) (fpcr : (BitVec 32)) (minimum : Bool) (pair : Bool) : (BitVec datasize) := Id.run do
   let result : (BitVec datasize) := (Zeros datasize)
@@ -831,7 +832,7 @@ def vector_arithmetic_binary_uniform_maxmin_fp_1985 (datasize : Nat) (elements :
     (pure loop_vars) ) : Id ((BitVec esize) × (BitVec esize) × (BitVec datasize)) )
   (pure result)
 
-/-- Type quantifiers: k_ex11403_ : Bool, k_ex11402_ : Bool, datasize : Nat, elements : Nat, esize :
+/-- Type quantifiers: k_ex12160_ : Bool, k_ex12159_ : Bool, datasize : Nat, elements : Nat, esize :
   Nat, esize ∈ {32, 64} ∧ elements ≥ 1 ∧ (elements * esize) = datasize -/
 def vector_arithmetic_binary_uniform_maxmin_fp_2008 (datasize : Nat) (elements : Nat) (esize : Nat) (operand1 : (BitVec datasize)) (operand2 : (BitVec datasize)) (fpcr : (BitVec 32)) (minimum : Bool) (pair : Bool) : (BitVec datasize) := Id.run do
   let result : (BitVec datasize) := (Zeros datasize)
@@ -881,7 +882,7 @@ def vector_arithmetic_unary_special_sqrt (datasize : Nat) (elements : Nat) (esiz
     (pure loop_vars) ) : Id ((BitVec esize) × (BitVec datasize)) )
   (pure result)
 
-/-- Type quantifiers: k_ex11550_ : Bool, datasize : Nat, elements : Nat, esize : Nat, esize ∈
+/-- Type quantifiers: k_ex12307_ : Bool, datasize : Nat, elements : Nat, esize : Nat, esize ∈
   {32, 64} ∧ elements ≥ 1 ∧ (elements * esize) = datasize -/
 def vector_arithmetic_unary_diffneg_fp (datasize : Nat) (elements : Nat) (esize : Nat) (operand : (BitVec datasize)) (neg : Bool) : (BitVec datasize) := Id.run do
   let result : (BitVec datasize) := (Zeros datasize)
@@ -1060,6 +1061,33 @@ def decode64_barrier_pure (op_code : (BitVec 32)) : (Bool × MemBarrierOp × MBR
       (if (((op_code &&& 0xFFFFF0FF#32) == 0xD50330DF#32) : Bool)
       then (system_barriers_decode_pure 0b10#2 CRm)
       else (false, MemBarrierOp_DSB, MBReqDomain_FullSystem, MBReqTypes_All)))
+
+def undefined_TLBIOperationTarget (_ : Unit) : SailM TLBIOperationTarget := do
+  (internal_pick [TLBIOperationTarget_VMALLS12E1IS])
+
+/-- Type quantifiers: arg_ : Nat, 0 ≤ arg_ ∧ arg_ ≤ 0 -/
+def TLBIOperationTarget_of_num (arg_ : Nat) : TLBIOperationTarget :=
+  match arg_ with
+  | _ => TLBIOperationTarget_VMALLS12E1IS
+
+def num_of_TLBIOperationTarget (arg_ : TLBIOperationTarget) : Int :=
+  match arg_ with
+  | .TLBIOperationTarget_VMALLS12E1IS => 0
+
+def aarch64_sysops_write_tlbi_target_pure (op0 : (BitVec 2)) (op1 : (BitVec 3)) (CRn : (BitVec 4)) (op2 : (BitVec 3)) (CRm : (BitVec 4)) : (Bool × TLBIOperationTarget) :=
+  if (((op0 == 0b01#2) && ((op1 == 0b100#3) && ((CRn == 0x8#4) && ((op2 == 0b110#3) && (CRm == 0x3#4))))) : Bool)
+  then (true, TLBIOperationTarget_VMALLS12E1IS)
+  else (false, TLBIOperationTarget_VMALLS12E1IS)
+
+def decode64_tlbi_target_pure (op_code : (BitVec 32)) : (Bool × TLBIOperationTarget) :=
+  let op0 : (BitVec 2) := (BitVec.slice op_code 19 2)
+  let op1 : (BitVec 3) := (BitVec.slice op_code 16 3)
+  let CRn : (BitVec 4) := (BitVec.slice op_code 12 4)
+  let CRm : (BitVec 4) := (BitVec.slice op_code 8 4)
+  let op2 : (BitVec 3) := (BitVec.slice op_code 5 3)
+  if (((op_code &&& 0xFFF80000#32) == 0xD5080000#32) : Bool)
+  then (aarch64_sysops_write_tlbi_target_pure op0 op1 CRn op2 CRm)
+  else (false, TLBIOperationTarget_VMALLS12E1IS)
 
 def initialize_registers (_ : Unit) : Unit :=
   ()
